cp

src/riot/x509/X509.ExtFields.BasicConstraints.fst
@@ -1,16 +1,10 @@
 module X509.ExtFields.BasicConstraints
 
-open LowParse.Spec.Base
-open LowParse.Spec.Combinators
-
-open ASN1.Base
 open ASN1.Spec
 open ASN1.Low
 
 open X509.Base
 open X509.BasicFields.Extension2
-
-module B32 = FStar.Bytes
 
 open FStar.Integers
 
@@ -66,27 +60,7 @@ open FStar.Integers
         pathLenConstraint       INTEGER (0..MAX) OPTIONAL }
  *)
 
-noextract inline_for_extraction
-let x509_basicConstraints_extValue_payload_t
-  (isCA: bool)
-= if isCA then
-  ( asn1_boolean_true_t `tuple2` (datatype_of_asn1_type INTEGER) )
-  else
-  ( asn1_boolean_false_t )
-
-let parse_x509_basicConstraints_extValue_payload_kind
-  (isCA: bool)
-: k: parser_kind {Mkparser_kind'?.parser_kind_subkind k == Some ParserStrong}
-= if isCA then
-  ( parse_asn1_TLV_kind_of_type BOOLEAN
-    `and_then_kind`
-    parse_asn1_TLV_kind_of_type INTEGER )
-  else
-  ( parse_asn1_TLV_kind_of_type BOOLEAN )
-
-let parse_x509_basicConstraints_extValue_payload
-  (isCA: bool)
-: parser (parse_x509_basicConstraints_extValue_payload_kind isCA) (x509_basicConstraints_extValue_payload_t isCA)
+let parse_x509_basicConstraints_extValue_payload isCA
 = if isCA then
   ( parse_asn1_boolean_TLV_true
     `nondep_then`
@@ -94,9 +68,7 @@ let parse_x509_basicConstraints_extValue_payload
   else
   ( parse_asn1_boolean_TLV_false )
 
-let serialize_x509_basicConstraints_extValue_payload
-  (isCA: bool)
-: serializer (parse_x509_basicConstraints_extValue_payload isCA)
+let serialize_x509_basicConstraints_extValue_payload isCA
 = if isCA then
   ( serialize_asn1_boolean_TLV_true
     `serialize_nondep_then`
@@ -104,10 +76,7 @@ let serialize_x509_basicConstraints_extValue_payload
   else
   ( serialize_asn1_boolean_TLV_false )
 
-noextract inline_for_extraction
-let serialize32_x509_basicConstraints_extValue_payload_backwards
-  (isCA: bool)
-: serializer32_backwards (serialize_x509_basicConstraints_extValue_payload isCA)
+let serialize32_x509_basicConstraints_extValue_payload_backwards isCA
 = if isCA then
   ( serialize32_asn1_boolean_TLV_true_backwards ()
     `serialize32_nondep_then_backwards`
@@ -115,20 +84,7 @@ let serialize32_x509_basicConstraints_extValue_payload_backwards
   else
   ( serialize32_asn1_boolean_TLV_false_backwards () )
 
-let lemma_serialize_x509_basicConstraints_extValue_payload_unfold
-  (isCA: bool)
-  (x: x509_basicConstraints_extValue_payload_t isCA)
-: Lemma (
-  serialize (serialize_x509_basicConstraints_extValue_payload isCA) x ==
-  ( if isCA then
-    ( let x = x <: asn1_boolean_true_t `tuple2` datatype_of_asn1_type INTEGER in
-      serialize (serialize_asn1_boolean_TLV_true) (fst x)
-      `Seq.append`
-      serialize (serialize_asn1_TLV_of_type INTEGER) (snd x) )
-    else
-    ( let x = x <: asn1_boolean_false_t in
-      serialize (serialize_asn1_boolean_TLV_false) x ) )
-)
+let lemma_serialize_x509_basicConstraints_extValue_payload_unfold isCA x
 = if isCA then
   ( serialize_nondep_then_eq
     (* s1 *) (serialize_asn1_boolean_TLV_true)
@@ -136,23 +92,6 @@ let lemma_serialize_x509_basicConstraints_extValue_payload_unfold
     (* in *) x )
   else
   ( () )
-
-let length_of_x509_basicConstraints_extValue_payload_hasLen
-  (pathLen: datatype_of_asn1_type INTEGER)
-: GTot (nat)
-= length_of_asn1_primitive_TLV true +
-  length_of_asn1_primitive_TLV pathLen
-
-let length_of_x509_basicConstraints_extValue_payload
-  (isCA: bool)
-: GTot ( if isCA then
-         ( datatype_of_asn1_type INTEGER -> GTot (asn1_value_length_of_type SEQUENCE) )
-         else
-         ( asn1_value_length_of_type SEQUENCE ) )
-= if isCA then
-  ( length_of_x509_basicConstraints_extValue_payload_hasLen )
-  else
-  ( length_of_asn1_primitive_TLV false )
 
 // let valid_x509_basicConstraints_extValue_payload
 //   (isCA: bool)
@@ -168,179 +107,56 @@ let length_of_x509_basicConstraints_extValue_payload
 //   else
 //   ( True )
 
-let len_of_x509_basicConstraints_extValue_payload_hasLen
-  (pathLen: datatype_of_asn1_type INTEGER)
-            // { valid_x509_basicConstraints_extValue_payload true pathLen })
-: Tot (len: asn1_value_int32_of_type SEQUENCE
-            { v len == length_of_x509_basicConstraints_extValue_payload_hasLen pathLen })
-= len_of_asn1_primitive_TLV true +
-  len_of_asn1_primitive_TLV pathLen
-
-noextract inline_for_extraction
-let len_of_x509_basicConstraints_extValue_payload
-  (isCA: bool)
-: Tot ( if isCA then
-         ( (pathLen: datatype_of_asn1_type INTEGER)
-           -> Tot (len: asn1_value_int32_of_type SEQUENCE
-                        { v len == length_of_x509_basicConstraints_extValue_payload true pathLen }) )
-         else
-         ( len: asn1_value_int32_of_type SEQUENCE
-                { v len == length_of_x509_basicConstraints_extValue_payload false } ) )
-= if isCA then
-  ( len_of_x509_basicConstraints_extValue_payload_hasLen )
-  else
-  ( len_of_asn1_primitive_TLV false )
-
-let lemma_serialize_x509_basicConstraints_extValue_payload_size
-  (isCA: bool)
-  (x: x509_basicConstraints_extValue_payload_t isCA)
-: Lemma (
-  Seq.length (serialize (serialize_x509_basicConstraints_extValue_payload isCA) x) ==
-  ( if isCA then
-    ( let x = x <: asn1_boolean_true_t `tuple2` datatype_of_asn1_type INTEGER in
-      length_of_x509_basicConstraints_extValue_payload true (snd x)  )
-    else
-    ( length_of_x509_basicConstraints_extValue_payload false ) )
-)
+let lemma_serialize_x509_basicConstraints_extValue_payload_size isCA x
 = lemma_serialize_x509_basicConstraints_extValue_payload_unfold isCA x
 
 (* extValue *)
 
-noextract inline_for_extraction
-let x509_basicConstraints_extValue_t
-  (isCA: bool)
-: Type
-= inbound_sequence_value_of
-  (**) (serialize_x509_basicConstraints_extValue_payload isCA)
-
-let parse_x509_basicConstraints_extValue
-  (isCA: bool)
-: parser _ (x509_basicConstraints_extValue_t isCA)
+let parse_x509_basicConstraints_extValue isCA
 = x509_basicConstraints_extValue_t isCA
   `coerce_parser`
   parse_asn1_sequence_TLV
   (**) (serialize_x509_basicConstraints_extValue_payload isCA)
 
-let serialize_x509_basicConstraints_extValue
-  (isCA: bool)
-: serializer (parse_x509_basicConstraints_extValue isCA)
+let serialize_x509_basicConstraints_extValue isCA
 = coerce_parser_serializer
     (parse_x509_basicConstraints_extValue isCA)
     (serialize_asn1_sequence_TLV
     (**) (serialize_x509_basicConstraints_extValue_payload isCA))
     ()
 
-noextract inline_for_extraction
-let serialize32_x509_basicConstraints_extValue_backwards
-  (isCA: bool)
-: serializer32_backwards (serialize_x509_basicConstraints_extValue isCA)
+let serialize32_x509_basicConstraints_extValue_backwards isCA
 = coerce_serializer32_backwards
     (serialize_x509_basicConstraints_extValue isCA)
     (serialize32_asn1_sequence_TLV_backwards
     (**) (serialize32_x509_basicConstraints_extValue_payload_backwards isCA))
     ()
 
-let lemma_serialize_x509_basicConstraints_extValue_unfold
-  (isCA: bool)
-  (x: x509_basicConstraints_extValue_t isCA)
-: Lemma (
-  predicate_serialize_asn1_sequence_TLV_unfold
-    (serialize_x509_basicConstraints_extValue_payload isCA)
-    (x)
-)
+let lemma_serialize_x509_basicConstraints_extValue_unfold isCA x
 = lemma_serialize_asn1_sequence_TLV_unfold
     (serialize_x509_basicConstraints_extValue_payload isCA)
     (x)
 
-let lemma_serialize_x509_basicConstraints_extValue_size
-  (isCA: bool)
-  (x: x509_basicConstraints_extValue_t isCA)
-: Lemma (
-  predicate_serialize_asn1_sequence_TLV_size
-    (serialize_x509_basicConstraints_extValue_payload isCA)
-    (x)
-)
+let lemma_serialize_x509_basicConstraints_extValue_size isCA x
 = lemma_serialize_asn1_sequence_TLV_size
     (serialize_x509_basicConstraints_extValue_payload isCA)
     (x)
 
-let length_of_x509_basicConstraints_extValue
-  (isCA: bool)
-: GTot ( if isCA then
-         ( datatype_of_asn1_type INTEGER -> GTot (asn1_value_length_of_type OCTET_STRING) )
-         else
-         ( asn1_value_length_of_type OCTET_STRING ) )
-= if isCA then
-  ( fun (pathLen: datatype_of_asn1_type INTEGER) ->
-      length_of_TLV
-        (SEQUENCE)
-        (length_of_x509_basicConstraints_extValue_payload true pathLen) )
-  else
-  ( length_of_TLV
-      (SEQUENCE)
-      (length_of_x509_basicConstraints_extValue_payload isCA) )
-
-noextract inline_for_extraction
-let len_of_x509_basicConstraints_extValue
-  (isCA: bool)
-: Tot ( if isCA then
-         ( (pathLen: datatype_of_asn1_type INTEGER)
-           -> Tot (len: asn1_value_int32_of_type OCTET_STRING
-                        { v len == length_of_x509_basicConstraints_extValue true pathLen }) )
-        else
-        ( len: asn1_value_int32_of_type OCTET_STRING
-               { v len == length_of_x509_basicConstraints_extValue isCA } ) )
-= if isCA then
-  ( fun (pathLen: datatype_of_asn1_type INTEGER) ->
-      len_of_TLV
-        (SEQUENCE)
-        (len_of_x509_basicConstraints_extValue_payload true pathLen) )
-  else
-  ( len_of_TLV
-      (SEQUENCE)
-      (len_of_x509_basicConstraints_extValue_payload isCA) )
-
-let lemma_serialize_x509_basicConstraints_extValue_size_exact
-  (isCA: bool)
-  (x: x509_basicConstraints_extValue_t isCA)
-: Lemma (
-  lemma_serialize_x509_basicConstraints_extValue_unfold isCA x;
-  lemma_serialize_x509_basicConstraints_extValue_size isCA x;
-    lemma_serialize_x509_basicConstraints_extValue_payload_size isCA x;
-  if isCA then
-  ( let x = x <: asn1_boolean_true_t `tuple2` datatype_of_asn1_type INTEGER in
-    length_of_opaque_serialization (serialize_x509_basicConstraints_extValue isCA) x
-    == length_of_x509_basicConstraints_extValue true (snd x) )
-  else
-  ( length_of_opaque_serialization (serialize_x509_basicConstraints_extValue isCA) x
-    == length_of_x509_basicConstraints_extValue false )
-)
+let lemma_serialize_x509_basicConstraints_extValue_size_exact isCA x
 = lemma_serialize_x509_basicConstraints_extValue_unfold isCA x;
   lemma_serialize_x509_basicConstraints_extValue_size isCA x;
     lemma_serialize_x509_basicConstraints_extValue_payload_size isCA x
 
 (* ext *)
 
-noextract inline_for_extraction
-let x509_basicConstraints_t
-  (isCA: bool)
-: Type
-= x509_extension_t
-  (**) (OID_BASIC_CONSTRAINTS)
-  (**) (serialize_x509_basicConstraints_extValue isCA)
-
-let parse_x509_basicConstraints
-  (isCA: bool)
-: parser parse_x509_extension_kind (x509_basicConstraints_t isCA)
+let parse_x509_basicConstraints isCA
 = x509_basicConstraints_t isCA
   `coerce_parser`
   parse_x509_extension
   (**) (OID_BASIC_CONSTRAINTS)
   (**) (serialize_x509_basicConstraints_extValue isCA)
 
-let serialize_x509_basicConstraints
-  (isCA: bool)
-: serializer (parse_x509_basicConstraints isCA)
+let serialize_x509_basicConstraints isCA
 = coerce_parser_serializer
     (parse_x509_basicConstraints isCA)
     (serialize_x509_extension
@@ -348,10 +164,7 @@ let serialize_x509_basicConstraints
     (**) (serialize_x509_basicConstraints_extValue isCA))
     ()
 
-noextract inline_for_extraction
-let serialize32_x509_basicConstraints_backwards
-  (isCA: bool)
-: serializer32_backwards (serialize_x509_basicConstraints isCA)
+let serialize32_x509_basicConstraints_backwards isCA
 = coerce_serializer32_backwards
     (_)
     (serialize32_x509_extension_backwards
@@ -359,97 +172,19 @@ let serialize32_x509_basicConstraints_backwards
     (**) (serialize32_x509_basicConstraints_extValue_backwards isCA))
     ()
 
-let lemma_serialize_x509_basicConstraints_unfold
-  (isCA: bool)
-  (x: x509_basicConstraints_t isCA)
-: Lemma ( predicate_serialize_x509_extension_unfold
-          (**) (OID_BASIC_CONSTRAINTS)
-          (**) (serialize_x509_basicConstraints_extValue isCA)
-          (**) (x) )
+let lemma_serialize_x509_basicConstraints_unfold isCA x
 = lemma_serialize_x509_extension_unfold
   (**) (OID_BASIC_CONSTRAINTS)
   (**) (serialize_x509_basicConstraints_extValue isCA)
   (**) (x)
 
-let lemma_serialize_x509_basicConstraints_size
-  (isCA: bool)
-  (x: x509_basicConstraints_t isCA)
-: Lemma ( predicate_serialize_x509_extension_size
-          (**) (OID_BASIC_CONSTRAINTS)
-          (**) (serialize_x509_basicConstraints_extValue isCA)
-          (**) (x) )
+let lemma_serialize_x509_basicConstraints_size isCA x
 = lemma_serialize_x509_extension_size
   (**) (OID_BASIC_CONSTRAINTS)
   (**) (serialize_x509_basicConstraints_extValue isCA)
   (**) (x)
 
-let length_of_x509_basicConstraints
-  (isCA: bool)
-: GTot ( if isCA then
-         ( datatype_of_asn1_type INTEGER -> GTot (asn1_TLV_length_of_type SEQUENCE) )
-         else
-         ( asn1_TLV_length_of_type SEQUENCE ) )
-= if isCA then
-  ( fun (pathLen: datatype_of_asn1_type INTEGER) ->
-      let x: x509_basicConstraints_extValue_payload_t isCA = (asn1_boolean_true, pathLen) in
-      lemma_serialize_x509_basicConstraints_extValue_size_exact isCA x;
-      lemma_serialize_x509_basicConstraints_extValue_payload_size isCA x;
-      length_of_x509_extension
-        (OID_BASIC_CONSTRAINTS)
-        (serialize_x509_basicConstraints_extValue isCA)
-        (x <: x509_basicConstraints_extValue_t isCA)
-        (length_of_x509_basicConstraints_extValue true pathLen) )
-  else
-  ( let x: x509_basicConstraints_extValue_payload_t isCA = (asn1_boolean_false) in
-    lemma_serialize_x509_basicConstraints_extValue_size_exact isCA x;
-    lemma_serialize_x509_basicConstraints_extValue_payload_size isCA x;
-    length_of_x509_extension
-      (OID_BASIC_CONSTRAINTS)
-      (serialize_x509_basicConstraints_extValue isCA)
-      (x <: x509_basicConstraints_extValue_t isCA)
-      (length_of_x509_basicConstraints_extValue false) )
-
-noextract inline_for_extraction
-let len_of_x509_basicConstraints
-  (isCA: bool)
-: Tot ( if isCA then
-         ( (pathLen: datatype_of_asn1_type INTEGER)
-           -> Tot (len: asn1_TLV_int32_of_type SEQUENCE
-                        { v len == length_of_x509_basicConstraints true pathLen }) )
-        else
-        ( len: asn1_TLV_int32_of_type SEQUENCE
-               { v len == length_of_x509_basicConstraints isCA } ) )
-= if isCA then
-  ( fun (pathLen: datatype_of_asn1_type INTEGER) ->
-      let x: x509_basicConstraints_extValue_payload_t isCA = (asn1_boolean_true, pathLen) in
-      lemma_serialize_x509_basicConstraints_extValue_size_exact isCA x;
-      lemma_serialize_x509_basicConstraints_extValue_payload_size isCA x;
-      len_of_x509_extension
-        (OID_BASIC_CONSTRAINTS)
-        (serialize_x509_basicConstraints_extValue isCA)
-        ((asn1_boolean_true, pathLen) <: x509_basicConstraints_extValue_payload_t isCA)
-        (len_of_x509_basicConstraints_extValue true pathLen) )
-  else
-  ( let x: x509_basicConstraints_extValue_payload_t isCA = (asn1_boolean_false) in
-    lemma_serialize_x509_basicConstraints_extValue_size_exact isCA x;
-    lemma_serialize_x509_basicConstraints_extValue_payload_size isCA x;
-    len_of_x509_extension
-      (OID_BASIC_CONSTRAINTS)
-      (serialize_x509_basicConstraints_extValue isCA)
-      (x <: x509_basicConstraints_extValue_t isCA)
-      (len_of_x509_basicConstraints_extValue false) )
-
-let lemma_serialize_x509_basicConstraints_size_exact
-  (isCA: bool)
-  (ext: x509_basicConstraints_t isCA)
-: Lemma (
-  length_of_opaque_serialization (serialize_x509_basicConstraints isCA) ext ==
-  ( if isCA then
-    ( let x = snd ext <: asn1_boolean_true_t `tuple2` datatype_of_asn1_type INTEGER in
-      length_of_x509_basicConstraints true (snd x) )
-    else
-    ( length_of_x509_basicConstraints false ) )
-)
+let lemma_serialize_x509_basicConstraints_size_exact isCA ext
 = if isCA then
   ( lemma_serialize_x509_basicConstraints_extValue_size_exact isCA (snd ext);
     lemma_serialize_x509_basicConstraints_extValue_payload_size isCA (snd ext);
@@ -457,7 +192,7 @@ let lemma_serialize_x509_basicConstraints_size_exact
       (OID_BASIC_CONSTRAINTS)
       (serialize_x509_basicConstraints_extValue isCA)
       (ext)
-      (length_of_x509_basicConstraints_extValue true (snd (snd ext <: x509_basicConstraints_extValue_payload_t true))) )
+      (v (len_of_x509_basicConstraints_extValue true (snd (snd ext <: x509_basicConstraints_extValue_payload_t true))) ))
   else
   ( lemma_serialize_x509_basicConstraints_extValue_size_exact isCA (snd ext);
     lemma_serialize_x509_basicConstraints_extValue_payload_size isCA (snd ext);
@@ -465,47 +200,7 @@ let lemma_serialize_x509_basicConstraints_size_exact
       (OID_BASIC_CONSTRAINTS)
       (serialize_x509_basicConstraints_extValue isCA)
       (ext)
-      (length_of_x509_basicConstraints_extValue false) )
-
-let x509_get_basicConstraints_isCA
-  (isCA: bool { isCA == true })
-  (criticality: datatype_of_asn1_type BOOLEAN)
-  (pathLen: datatype_of_asn1_type INTEGER)
-: Tot (x509_basicConstraints_t isCA)
-= let extValue_payload: x509_basicConstraints_extValue_payload_t isCA = ((isCA <: asn1_boolean_true_t), pathLen) in
-  (* Prf *) lemma_serialize_x509_basicConstraints_extValue_payload_size isCA extValue_payload;
-
-  let extValue: x509_basicConstraints_extValue_t isCA = extValue_payload in
-  (* Prf *) lemma_serialize_x509_basicConstraints_extValue_size_exact isCA extValue;
-
-  let ext: x509_basicConstraints_t isCA = x509_get_extension
-                                            (OID_BASIC_CONSTRAINTS)
-                                            (serialize_x509_basicConstraints_extValue isCA)
-                                            (extValue)
-                                            (len_of_x509_basicConstraints_extValue true pathLen)
-                                            (criticality)
-                                            in
-  (* return *) ext
-
-noextract inline_for_extraction
-let x509_get_basicConstraints_isNotCA
-  (isCA: bool { isCA == false })
-  (criticality: datatype_of_asn1_type BOOLEAN)
-: Tot (x509_basicConstraints_t isCA)
-= let extValue_payload: x509_basicConstraints_extValue_payload_t isCA = isCA <: asn1_boolean_false_t in
-  (* Prf *) lemma_serialize_x509_basicConstraints_extValue_payload_size isCA extValue_payload;
-
-  let extValue: x509_basicConstraints_extValue_t isCA = extValue_payload in
-  (* Prf *) lemma_serialize_x509_basicConstraints_extValue_size_exact isCA extValue;
-
-  let ext: x509_basicConstraints_t isCA = x509_get_extension
-                                            (OID_BASIC_CONSTRAINTS)
-                                            (Ghost.hide (serialize_x509_basicConstraints_extValue isCA))
-                                            (extValue)
-                                            (len_of_x509_basicConstraints_extValue isCA)
-                                            (criticality)
-                                            in
-  (* return *) ext
+      (v (len_of_x509_basicConstraints_extValue false) ))
 
 (* FIXME: Does not type check for some reason *)
 (*
